Various cleanups

theories/BasicAst.v
@@ -3,6 +3,8 @@ From LogRel.AutoSubst Require Import core unscoped.
 
 Record aname := { nNamed : string }.
 
+Definition anDummy := {| nNamed := "" |}.
+
 Definition eq_binder_annot (a a' : aname) := True.
 
 Inductive sort :=
