theories/LogicalRelation/Irrelevance.v
@@ -1,301 +1,248 @@
 From LogRel.AutoSubst Require Import core unscoped Ast Extra.
-From LogRel Require Import Notations Utils BasicAst Context Untyped Weakening GenericTyping LogicalRelation DeclarativeInstance.
-From LogRel.LogicalRelation Require Import Induction ShapeView Reflexivity.
+From LogRel Require Import Notations Utils BasicAst Context Untyped Weakening GenericTyping LogicalRelation.
+From LogRel.LogicalRelation Require Import Induction ShapeView Reflexivity Escape.
 
 Set Universe Polymorphism.
+Set Printing Universes.
 
 Section Irrelevances.
 Context `{GenericTypingProperties}.
 
-Section ΠIrrelevanceLemmas.
-Universe u u' v.
-Context Γ A A' (ΠA : PiRedTy@{u} Γ A) (ΠA' : PiRedTy@{u'} Γ A')
-  (dom := PiRedTy.dom ΠA)
-  (dom' := PiRedTy.dom ΠA')
-  (domRed := (@PiRedTy.domRed _ _ _ _ _ _ _ ΠA))
-  (domRed' := (@PiRedTy.domRed _ _ _ _ _ _ _ ΠA'))
-  (cod := PiRedTy.cod ΠA)
-  (cod' := PiRedTy.cod ΠA')
-  (codRed := (@PiRedTy.codRed _ _ _ _ _ _ _ ΠA))
-  (codRed' := (@PiRedTy.codRed _ _ _ _ _ _ _ ΠA'))
-  (eqPi : [Γ |- tProd (PiRedTy.na ΠA) dom cod ≅ tProd (PiRedTy.na ΠA') dom' cod']).
+Section EquivLRPack.
+  Universe i i' v.
 
-Notation "A <≈> B" := (prod@{v v} (A -> B) (B -> A)) (at level 90).
+  Notation "A <≈> B" := (prod@{v v} (A -> B) (B -> A)) (at level 90).
 
-Lemma ΠIrrelevanceTyEq  :
-  (forall (Δ : context) (ρ : Δ ≤ Γ) (h : [  |- Δ]),
-  (and3@{v v v} (forall B : term,
-      [domRed Δ ρ h | Δ ||- dom⟨ρ⟩ ≅ B] <≈> [domRed' Δ ρ h | Δ ||- dom'⟨ρ⟩ ≅ B])
-    (forall t : term,
-      [domRed Δ ρ h | Δ ||- t : dom⟨ρ⟩] <≈> [domRed' Δ ρ h | Δ ||- t : dom'⟨ρ⟩])
-    (forall t u : term,
-      [domRed Δ ρ h | Δ ||- t ≅ u : dom⟨ρ⟩ ] <≈> [domRed' Δ ρ h | Δ ||- t ≅ u : dom'⟨ρ⟩]))) ->
-  (forall (Δ : context) (ρ : Δ ≤ Γ) (a : term) (h : [  |- Δ])
-      (ha : [domRed Δ ρ h | Δ ||- a : dom⟨ρ⟩])
-      (ha' : [domRed' Δ ρ h | Δ ||- a : dom'⟨ρ⟩]),
-  (and3@{v v v} (forall B : term,
-      [codRed Δ a ρ h ha | Δ ||- cod[a .: (ρ >> tRel)] ≅ B] <≈>
-      [codRed' Δ a ρ h ha' | Δ ||- cod'[a .: (ρ >> tRel)] ≅ B])
-    (forall t : term,
-      [codRed Δ a ρ h ha | Δ ||- t : cod[a .: (ρ >> tRel)] ] <≈>
-      [codRed' Δ a ρ h ha' | Δ ||- t : cod'[a .: (ρ >> tRel)]])
-    (forall t u : term,
-      [codRed Δ a ρ h ha | Δ ||- t ≅ u : cod[a .: (ρ >> tRel)]] <≈>
-      [codRed' Δ a ρ h ha' | Δ ||- t ≅ u : cod'[a .: (ρ >> tRel)] ]))) ->
-  forall B, [Γ ||-Π A ≅ B | ΠA] -> [Γ ||-Π A' ≅ B | ΠA'].
+  Definition equivLRPack {Γ Γ' A A'} (P: LRPack@{i} Γ A) (P': LRPack@{i'} Γ' A'):=
+    and3@{v v v} 
+      (forall B, [P | Γ ||- A ≅ B] <≈> [P' | Γ' ||- A' ≅ B])
+      (forall t, [P | Γ ||- t : A] <≈> [P' | Γ' ||- t : A'])
+      (forall t u, [P | Γ ||- t ≅ u : A] <≈> [P' | Γ' ||- t ≅ u : A']).
+End EquivLRPack.
+
+Lemma symLRPack@{i i' v} {Γ Γ' A A'} {P: LRPack@{i} Γ A} {P': LRPack@{i'} Γ' A'} :
+    equivLRPack@{i i' v} P P' -> equivLRPack@{i' i v} P' P.
 Proof.
-  intros IHdom IHcod B [] ; cbn in *.
-  econstructor.
+  intros [eqT rTm eqTm]; constructor;split ;
+    apply eqT + apply rTm + apply eqTm.
+Qed.
+  
+
+Section ΠIrrelevanceLemmas.
+Universe i j k l i' j' k' l' v.
+Context {Γ lA A lA' A'} 
+  (ΠA : PiRedTyPack@{i j k l} Γ A lA) 
+  (ΠA' : PiRedTyPack@{i' j' k' l'} Γ A' lA')
+  (RA := LRPi' ΠA)
+  (RA' := LRPi' ΠA')
+  (domRed := (@PiRedTyPack.domRed _ _ _ _ _ _ _ _ _ _ _ _ ΠA))
+  (domRed' := (@PiRedTyPack.domRed _ _ _ _ _ _ _ _ _ _ _ _  ΠA'))
+  (codRed := (@PiRedTyPack.codRed  _ _ _ _ _ _ _ _ _ _ _ _ ΠA))
+  (codRed' := (@PiRedTyPack.codRed  _ _ _ _ _ _ _ _ _ _ _ _  ΠA'))
+  (eqPi : [Γ |- PiRedTyPack.prod ΠA ≅ PiRedTyPack.prod ΠA']).
+
+Context (eqvDom : forall {Δ} (ρ : Δ ≤ Γ) (wfΔ : [  |- Δ]),
+          equivLRPack@{k k' v} (domRed Δ ρ wfΔ) (domRed' Δ ρ wfΔ))
+        (eqvCod : forall {Δ a} (ρ : Δ ≤ Γ) (wfΔ : [  |- Δ])
+          (ha : [domRed Δ ρ wfΔ| Δ ||- a : _])
+          (ha' : [domRed' Δ ρ wfΔ | Δ ||- a : _]),
+          equivLRPack@{k k' v} (codRed Δ a ρ wfΔ ha) (codRed' Δ a ρ wfΔ ha')).
+
+Lemma ΠIrrelevanceTyEq B : [Γ ||-<lA> A ≅ B | RA] -> [Γ ||-<lA'> A' ≅ B | RA'].
+Proof.
+  intros [] ; cbn in *; econstructor.
   - now gen_typing.
-  - cbn in *.
-    etransitivity.
-    2: eassumption.
-    now symmetry.
-  - intros ; now apply IHdom.
-  - intros.
-    cbn in *.
-    unshelve eapply IHcod.
+  - cbn; etransitivity; [|tea]; now symmetry.
+  - intros ; now apply eqvDom.
+  - intros; cbn; unshelve eapply eqvCod.
     2: eauto.
-    now eapply IHdom.
+    now eapply eqvDom.
 Qed.
 
-Lemma ΠIrrelevanceTm  :
-  (forall (Δ : context) (ρ : Δ ≤ Γ) (h : [  |- Δ]),
-  (and3@{v v v} (forall B : term,
-      [domRed Δ ρ h | Δ ||- dom⟨ρ⟩ ≅ B] <≈> [domRed' Δ ρ h | Δ ||- dom'⟨ρ⟩ ≅ B])
-    (forall t : term,
-      [domRed Δ ρ h | Δ ||- t : dom⟨ρ⟩] <≈> [domRed' Δ ρ h | Δ ||- t : dom'⟨ρ⟩])
-    (forall t u : term,
-      [domRed Δ ρ h | Δ ||- t ≅ u : dom⟨ρ⟩ ] <≈> [domRed' Δ ρ h | Δ ||- t ≅ u : dom'⟨ρ⟩]))) ->
-  (forall (Δ : context) (ρ : Δ ≤ Γ) (a : term) (h : [  |- Δ])
-      (ha : [domRed Δ ρ h | Δ ||- a : dom⟨ρ⟩])
-      (ha' : [domRed' Δ ρ h | Δ ||- a : dom'⟨ρ⟩]),
-  (and3@{v v v} (forall B : term,
-      [codRed Δ a ρ h ha | Δ ||- cod[a .: (ρ >> tRel)] ≅ B] <≈>
-      [codRed' Δ a ρ h ha' | Δ ||- cod'[a .: (ρ >> tRel)] ≅ B])
-    (forall t : term,
-      [codRed Δ a ρ h ha | Δ ||- t : cod[a .: (ρ >> tRel)] ] <≈>
-      [codRed' Δ a ρ h ha' | Δ ||- t : cod'[a .: (ρ >> tRel)]])
-    (forall t u : term,
-      [codRed Δ a ρ h ha | Δ ||- t ≅ u : cod[a .: (ρ >> tRel)]] <≈>
-      [codRed' Δ a ρ h ha' | Δ ||- t ≅ u : cod'[a .: (ρ >> tRel)] ]))) ->
-  forall t, [Γ ||-Π t : A | ΠA] -> [Γ ||-Π t : A' | ΠA'].
+Lemma ΠIrrelevanceTm t : [Γ ||-<lA> t : A | RA] -> [Γ ||-<lA'> t : A' | RA'].
 Proof.
-  intros IHdom IHcod B [] ; cbn in *.
-  econstructor.
-  - cbn.
-    econstructor.
-    all: gen_typing.
-  - eassumption.
-  - cbn.
-    gen_typing.
-  - intros.
-    unshelve eapply IHcod.
+  intros []; cbn in *; econstructor; tea.
+  - now eapply redtmwf_conv.
+  - now eapply convtm_conv.
+  - intros; unshelve eapply eqvCod.
     2: now auto.
-    now apply IHdom.
-  - intros.
-    unshelve eapply IHcod, eq.
-    all: now eapply IHdom.
+    now apply eqvDom.
+  - intros; unshelve eapply eqvCod, eq.
+    all: now eapply eqvDom.
 Defined.
 
-Lemma ΠIrrelevanceTmEq  :
-  (forall (Δ : context) (ρ : Δ ≤ Γ) (h : [  |- Δ]),
-  (and3@{v v v} (forall B : term,
-      [domRed Δ ρ h | Δ ||- dom⟨ρ⟩ ≅ B] <≈> [domRed' Δ ρ h | Δ ||- dom'⟨ρ⟩ ≅ B])
-    (forall t : term,
-      [domRed Δ ρ h | Δ ||- t : dom⟨ρ⟩] <≈> [domRed' Δ ρ h | Δ ||- t : dom'⟨ρ⟩])
-    (forall t u : term,
-      [domRed Δ ρ h | Δ ||- t ≅ u : dom⟨ρ⟩ ] <≈> [domRed' Δ ρ h | Δ ||- t ≅ u : dom'⟨ρ⟩]))) ->
-  (forall (Δ : context) (ρ : Δ ≤ Γ) (a : term) (h : [  |- Δ])
-      (ha : [domRed Δ ρ h | Δ ||- a : dom⟨ρ⟩])
-      (ha' : [domRed' Δ ρ h | Δ ||- a : dom'⟨ρ⟩]),
-  (and3@{v v v} (forall B : term,
-      [codRed Δ a ρ h ha | Δ ||- cod[a .: (ρ >> tRel)] ≅ B] <≈>
-      [codRed' Δ a ρ h ha' | Δ ||- cod'[a .: (ρ >> tRel)] ≅ B])
-    (forall t : term,
-      [codRed Δ a ρ h ha | Δ ||- t : cod[a .: (ρ >> tRel)] ] <≈>
-      [codRed' Δ a ρ h ha' | Δ ||- t : cod'[a .: (ρ >> tRel)]])
-    (forall t u : term,
-      [codRed Δ a ρ h ha | Δ ||- t ≅ u : cod[a .: (ρ >> tRel)]] <≈>
-      [codRed' Δ a ρ h ha' | Δ ||- t ≅ u : cod'[a .: (ρ >> tRel)] ]))) ->
-  forall t u, [Γ ||-Π t ≅ u : A | ΠA] -> [Γ ||-Π t ≅ u : A' | ΠA'].
+Lemma ΠIrrelevanceTmEq t u : [Γ ||-<lA> t ≅ u : A | RA] -> [Γ ||-<lA'> t ≅ u : A' | RA'].
 Proof.
-  intros IHdom IHcod t u [] ; cbn in *.
-  unshelve econstructor.
-  - now eapply ΠIrrelevanceTm.
-  - now eapply ΠIrrelevanceTm.
-  - cbn.
-    gen_typing.
-  - intros.
-    unshelve eapply IHcod.
+  intros [] ; cbn in *; unshelve econstructor.
+  1,2: now eapply ΠIrrelevanceTm.
+  - now eapply convtm_conv.
+  - intros; unshelve eapply eqvCod.
     2: now auto.
-    now apply IHdom.
+    now apply eqvDom.
 Qed.
 
 End ΠIrrelevanceLemmas.
+
+Lemma ΠIrrelevanceLRPack@{i j k l i' j' k' l' v}
+  {Γ lA A lA' A'} 
+  (ΠA : PiRedTyPack@{i j k l} Γ A lA) 
+  (ΠA' : PiRedTyPack@{i' j' k' l'} Γ A' lA')
+  (RA := LRPi' ΠA)
+  (RA' := LRPi' ΠA')
+  (domRed := (@PiRedTyPack.domRed _ _ _ _ _ _ _ _ _ _ _ _ ΠA))
+  (domRed' := (@PiRedTyPack.domRed _ _ _ _ _ _ _ _ _ _ _ _  ΠA'))
+  (codRed := (@PiRedTyPack.codRed  _ _ _ _ _ _ _ _ _ _ _ _ ΠA))
+  (codRed' := (@PiRedTyPack.codRed  _ _ _ _ _ _ _ _ _ _ _ _  ΠA'))
+  (eqPi : [Γ |- PiRedTyPack.prod ΠA ≅ PiRedTyPack.prod ΠA'])
+  (eqvDom : forall {Δ} (ρ : Δ ≤ Γ) (wfΔ : [  |- Δ]),
+          equivLRPack@{k k' v} (domRed Δ ρ wfΔ) (domRed' Δ ρ wfΔ))
+  (eqvCod : forall {Δ a} (ρ : Δ ≤ Γ) (wfΔ : [  |- Δ])
+          (ha : [Δ ||-<lA> a : _| domRed Δ ρ wfΔ])
+          (ha' : [Δ ||-<lA'> a : _| domRed' Δ ρ wfΔ ]),
+          equivLRPack@{k k' v} (codRed Δ a ρ wfΔ ha) (codRed' Δ a ρ wfΔ ha'))
+  : equivLRPack@{k k' v} RA RA'.
+Proof.
+  pose proof (eqvDom' := fun Δ ρ wfΔ => symLRPack (@eqvDom Δ ρ wfΔ)).
+  pose proof (eqvCod' := fun Δ a ρ wfΔ ha ha' => symLRPack (@eqvCod Δ a ρ wfΔ ha ha')).
+  constructor.
+  - split; now apply ΠIrrelevanceTyEq.
+  - split; now apply ΠIrrelevanceTm.
+  - split; now apply ΠIrrelevanceTmEq.
+Qed.
+
+Set Printing Primitive Projection Parameters.
+
+Lemma NeIrrelevanceLRPack@{i j k l i' j' k' l' v}
+  {Γ A A'} lA lA'
+  (neA : [Γ ||-ne A])
+  (neA' : [Γ ||-ne A'])
+  (RA := LRne_@{i j k l} lA neA)
+  (RA' := LRne_@{i' j' k' l'} lA' neA')
+  (eqAA' : [Γ ||-ne A ≅ A' | neA ])
+  : equivLRPack@{k k' v} RA RA'.
+Proof.
+  destruct neA as [ty], neA' as [ty'], eqAA' as [ty0']; cbn in *.
+  assert (ty0' = ty') by (eapply redtywf_det; tea; now constructor); subst.
+  assert [Γ |- ty ≅ ty'] as convty by gen_typing.
+  split.
+  + intros ?; split; intros []; econstructor; cbn in *; tea.
+    all: etransitivity ; [| tea]; tea; now symmetry.
+  + intros ?; split; intros []; econstructor; cbn in *; tea.
+    1,3: now eapply redtmwf_conv.
+    all: now eapply convneu_conv.
+  + intros ??; split; intros []; econstructor; cbn in *.
+    1-2,6-7: now eapply redtmwf_conv.
+    all: tea.
+    all: now eapply convneu_conv.
+Qed.
+
+
+Lemma NeNfconv {Γ k A A'} : [Γ |- A ≅ A'] -> [Γ ||-NeNf k : A] -> [Γ ||-NeNf k : A'].
+Proof.
+  intros ? []; econstructor; tea; gen_typing.
+Qed.
+
+Lemma NeNfEqconv {Γ k k' A A'} : [Γ |- A ≅ A'] -> [Γ ||-NeNf k ≅ k' : A] -> [Γ ||-NeNf k ≅ k' : A'].
+Proof.
+  intros ? []; econstructor; tea; gen_typing.
+Qed.
+
 
 Section LRIrrelevant.
 Universe u v. (* u is a small universe level that may be instanciated to Set. v is a large universe level *)
 
 Notation "A <≈> B" := (prod@{v v} (A -> B) (B -> A)) (at level 90).
 
-Lemma LRIrrelevantPreds@{i j k l i' j' k' l'} {lA lA'}
-  (IH : forall l0 (ltA : l0 << lA) (ltA' : l0 << lA')
-    , prod@{v v}
+Section LRIrrelevantInductionStep.
+
+Universe i j k l i' j' k' l'.
+
+Definition IHStatement lA lA' :=
+  (forall l0 (ltA : l0 << lA) (ltA' : l0 << lA'),
+      prod@{v v}
         (forall Γ t, [ LogRelRec@{i j k} lA l0 ltA | Γ ||- t ] <≈> [ LogRelRec@{i' j' k'} lA' l0 ltA' | Γ ||- t ])
-        (forall Γ t (lr1 : [ LogRelRec@{i j k} lA l0 ltA | Γ ||- t ])
-                (lr2 : [ LogRelRec@{i' j' k'} lA' l0 ltA' | Γ ||- t ]) u
-          , [ LogRelRec@{i j k} lA l0 ltA | Γ ||- t ≅ u | lr1 ] <≈> [ LogRelRec@{i' j' k'} lA' l0 ltA' | Γ ||- t ≅ u | lr2 ]))
+        (forall Γ t
+           (lr1 : [ LogRelRec@{i j k} lA l0 ltA | Γ ||- t ])
+           (lr2 : [ LogRelRec@{i' j' k'} lA' l0 ltA' | Γ ||- t ])
+           u,
+            [ LogRelRec@{i j k} lA l0 ltA | Γ ||- t ≅ u | lr1 ] <≈>
+            [ LogRelRec@{i' j' k'} lA' l0 ltA' | Γ ||- t ≅ u | lr2 ])).
+
+Lemma UnivIrrelevanceLRPack
+  {Γ lA lA' A A'}
+  (IH : IHStatement lA lA')
+  (hU : [Γ ||-U<lA> A]) (hU' : [Γ ||-U<lA'> A'])
+  (RA := LRU_@{i j k l} hU) (RA' := LRU_@{i' j' k' l'} hU') :
+  equivLRPack@{k k' v} RA RA'.
+Proof.
+  revert IH; destruct hU as [_ []], hU' as [_ []]; intro IH; destruct (IH zero Oi Oi) as [IHty IHeq].
+  constructor.
+  + intros; cbn; split; intros []; now constructor.
+  + intros ?; destruct (IHty Γ t) as [tfwd tbwd]; split; intros [];
+      unshelve econstructor.
+    6: now apply tfwd.
+    9: now apply tbwd.
+    all : tea.
+  + cbn ; intros ? ?;
+    destruct (IHty Γ t) as [tfwd tbwd];
+    destruct (IHty Γ u) as [ufwd ubwd].
+    split; intros [[] []]; cbn in *; unshelve econstructor.
+    3: now apply tfwd.
+    5: now apply tbwd.
+    6: now apply ufwd.
+    8: now apply ubwd.
+    (* all: apply todo. *)
+    all: cbn.
+    6: now refine (fst (IHeq _ _ _ _ _) _).
+    7: now refine (snd (IHeq _ _ _ _ _) _).
+    1-4: now econstructor.
+    all: cbn; tea.
+Qed.
+
+Lemma LRIrrelevantPreds {lA lA'}
+  (IH : IHStatement lA lA')
   (Γ : context) (A A' : term)
   {eqTyA redTmA : term -> Type@{k}}
   {eqTyA' redTmA' : term -> Type@{k'}}
   {eqTmA : term -> term -> Type@{k}}
   {eqTmA' : term -> term -> Type@{k'}}
   (lrA : LogRel@{i j k l} lA Γ A eqTyA redTmA eqTmA)
-  (lrA' : LogRel@{i' j' k' l'} lA' Γ A' eqTyA' redTmA' eqTmA') :
+  (lrA' : LogRel@{i' j' k' l'} lA' Γ A' eqTyA' redTmA' eqTmA')
+  (RA := Build_LRPack Γ A eqTyA redTmA eqTmA)
+  (RA' := Build_LRPack Γ A' eqTyA' redTmA' eqTmA') :
   eqTyA A' ->
-  @and3@{v v v} (forall B, eqTyA B <≈> eqTyA' B)
-    (forall t, redTmA t <≈> redTmA' t)
-    (forall t u, eqTmA t u <≈> eqTmA' t u).
+  equivLRPack@{k k' v} RA RA'.
 Proof.
   pose proof (fun Γ l0 ltA ltA' => fst (IH l0 ltA ltA') Γ) as IHty.
   pose proof (fun Γ l0 ltA ltA' => snd (IH l0 ltA ltA') Γ) as IHeq.
   intros he.
   set (s := ShapeViewConv lrA lrA' he).
-  induction lrA as [? ? [l1 lt1] | ? ? [] | ? A [] [] IHdom IHcod]
-    in A', eqTyA', eqTmA', redTmA', lrA', he, s |- *.
-  - destruct lrA' as [? ? [l2 lt2] | | ]; try solve [destruct s] ; clear s.
-    destruct lt2 ; destruct lt1. split.
-    + intros ?.
-      split.
-      all: eauto.
-    + intros ?.
-      split.
-      all: intros [].
-      all: econstructor.
-      1, 2, 3, 5, 6, 7: tea.
-      * apply (fst (IHty Γ zero Oi Oi t)). exact rel.
-      * apply (snd (IHty Γ zero Oi Oi t)). exact rel.
-    + cbn ; intros ? ?.
-      split.
-      all: intros [[] []] ; cbn in *.
-      all: unshelve econstructor.
-      * econstructor. 1, 2, 3: tea.
-        apply (fst (IHty Γ zero Oi Oi t)). exact relL.
-      * econstructor. 1, 2, 3: tea.
-        apply (fst (IHty Γ zero Oi Oi u)). exact relR.
-      * apply (fst (IHty Γ zero Oi Oi t)). exact relL.
-      * econstructor. 1, 2, 3: tea.
-        apply (snd (IHty Γ zero Oi Oi t)). exact relL.
-      * econstructor. 1, 2, 3: tea.
-        apply (snd (IHty Γ zero Oi Oi u)). exact relR.
-      * apply (snd (IHty Γ zero Oi Oi t)). exact relL.
-      * cbn. eassumption.
-      * apply (fst (IHty Γ zero Oi Oi u)). exact relR.
-      * apply (fst (IHeq Γ zero Oi Oi t relL (fst (IHty Γ zero Oi Oi t) relL) u)). exact relEq.
-      * cbn. eassumption.
-      * apply (snd (IHty Γ zero Oi Oi u)). exact relR.
-      * apply (snd (IHeq Γ zero Oi Oi t (snd (IHty Γ zero Oi Oi t) relL) relL u)). exact relEq.
-  - destruct lrA' as [|? A' neA'|] ; try solve [destruct s] ; clear s.
-    destruct he as [AA], neA' as [AA'] ; cbn in *.
-    assert (AA' = AA) as eqAA'.
-    {
-      all: eapply whredty_det ; econstructor ; [idtac |now econstructor| idtac |now econstructor].
-      all: gen_typing.
-    }
-    revert red1 ne1 eq1. pattern AA'.
-    set (P := fun _ => _). apply (tr P (eq_sym eqAA')). subst P; cbn.
-    intros red1 ne1 eq1.
-    assert [Γ |- ty ≅ AA] as convtAA by gen_typing.
-    split.
-    + intros ?.
-      split.
-      all: intros [].
-      all: econstructor.
-      all: cbn in *.
-      all: try eauto.
-      2: etransitivity ; eassumption.
-      clear eq1; etransitivity ; [symmetry|..]; eassumption.
-    + intros ?.
-      split.
-      2: symmetry in convtAA.
-      all: intros [].
-      all: econstructor ; cbn in *.
-      all: try eauto.
-      1,3: eapply redtmwf_conv ; eassumption.
-      all: gen_typing.
-    + intros ? ?.
-      split.
-      2: symmetry in convtAA.
-      all: intros [].
-      all: econstructor.
-      all: cbn in *.
-      1-2,6-7: eapply redtmwf_conv ; eassumption.
-      1-2,4-5: eassumption.
-      all: now gen_typing.
-  - destruct lrA' as [| | ? A' [] []] ; try solve [destruct s] ; clear s.
-    destruct he ; cbn -[subst1] in *.
+  induction lrA as [? ? h1 | ? ? neA | ? A ΠA HAad IHdom IHcod]
+    in RA, A', RA', eqTyA', eqTmA', redTmA', lrA', he, s |- *.
+  - destruct lrA' as [? ? h2 | | ]; try solve [destruct s] ; clear s.
+    now apply UnivIrrelevanceLRPack.
+  - destruct lrA' as [|? A' neA'| ] ; try solve [destruct s] ; clear s.
+    exact (NeIrrelevanceLRPack lA lA' neA neA' he).
+  - destruct lrA' as [| | ? A' ΠA' HAad'] ; try solve [destruct s] ; clear s.
+    pose (PA := PiRedTyPack.pack ΠA HAad).
+    pose (PA' := PiRedTyPack.pack ΠA' HAad').
+    destruct he as [na0 dom0 cod0 ?? domRed codRed], ΠA' as [na1 dom1 cod1];
     assert (tProd na0 dom0 cod0 = tProd na1 dom1 cod1) as ePi
-      by (eapply whredty_det ; gen_typing).
+    by (eapply whredty_det ; gen_typing).
     inversion ePi ; subst ; clear ePi.
-    pose proof (IHdom_ := fun Δ ρ h => IHdom Δ ρ h _ _ _ _ (domAd0 Δ ρ h) (domRed1 Δ ρ h)).
-    assert (IHcod_ : forall Δ a (ρ : Δ ≤ Γ) (h : [|- Δ])
-      (ha : [domRed Δ ρ h | Δ ||- a : dom⟨ρ⟩])
-      (ha' : [domRed0 Δ ρ h | Δ ||- a : dom1⟨ρ⟩]),
-      [×
-        (forall B,
-          [codRed Δ a ρ h ha | Δ ||- cod[a .: (ρ >> tRel)] ≅ B] <≈>
-          [codRed0 Δ a ρ h ha' | Δ ||- cod1[a .: (ρ >> tRel)] ≅ B]),
-        (forall t,
-          [codRed Δ a ρ h ha | Δ ||- t : cod[a .: (ρ >> tRel)]] <≈>
-          [codRed0 Δ a ρ h ha' | Δ ||- t : cod1[a .: (ρ >> tRel)]]) &
-      (forall t u,
-        [codRed Δ a ρ h ha | Δ ||- t ≅ u : cod[a .: (ρ >> tRel)]] <≈>
-        [codRed0 Δ a ρ h ha' | Δ ||- t ≅ u : cod1[a .: (ρ >> tRel)]])
-      ]).
-    {
-      intros.
-      eapply IHcod.
-      1: eapply codAd0.
-      eauto.
-    }
-    split.
-    + split ; intros.
-      all: eapply ΠIrrelevanceTyEq.
-      4,8: eassumption.
-      1,4: assumption + now symmetry.
-      1-2: now eauto.
-      * do 2 split ; intros.
-        all: now eapply IHdom_ ; eauto.
-      * do 2 split ; intros.
-        all: now eapply IHcod_ ; eauto.
-    + split ; intros.
-      all: eapply ΠIrrelevanceTm.
-      4,8: eassumption.
-      1,4: assumption + now symmetry.
-      1-2: now eauto.
-      * do 2 split ; intros.
-        all: now eapply IHdom_ ; eauto.
-      * do 2 split ; intros.
-        all: now eapply IHcod_ ; eauto.
-    + split ; intros.
-      all: eapply ΠIrrelevanceTmEq.
-      4,8: eassumption.
-      1,4: assumption + now symmetry.
-      1-2: now eauto.
-      * do 2 split ; intros.
-        all: now eapply IHdom_ ; eauto.
-      * do 2 split ; intros.
-        all: now eapply IHcod_ ; eauto.
+    eapply (ΠIrrelevanceLRPack PA PA').
+    + eassumption.
+    + intros; unshelve eapply IHdom.
+      1: eapply (LRAd.adequate (PiRedTyPack.domRed PA' _ _)).
+      eapply domRed.
+    + intros; unshelve eapply IHcod.
+      1: eapply (LRAd.adequate (PiRedTyPack.codRed PA' _ _ _)).
+      eapply codRed.
 Qed.
 
-Lemma LRIrrelevantCumTy@{i j k l i' j' k' l'} {lA}
-  (IH : forall l0 (ltA : l0 << lA) (ltA' : l0 << lA)
-    , prod@{v v}
-        (forall Γ t, [ LogRelRec@{i j k} lA l0 ltA | Γ ||- t ] <≈> [ LogRelRec@{i' j' k'} lA l0 ltA' | Γ ||- t ])
-        (forall Γ t (lr1 : [ LogRelRec@{i j k} lA l0 ltA | Γ ||- t ])
-                (lr2 : [ LogRelRec@{i' j' k'} lA l0 ltA' | Γ ||- t ]) u
-          , [ LogRelRec@{i j k} lA l0 ltA | Γ ||- t ≅ u | lr1 ] <≈> [ LogRelRec@{i' j' k'} lA l0 ltA' | Γ ||- t ≅ u | lr2 ]))
+
+Lemma LRIrrelevantCumTy {lA}
+  (IH : IHStatement lA lA)
   (Γ : context) (A : term)
   : [ LogRel@{i j k l} lA | Γ ||- A ] -> [ LogRel@{i' j' k' l'} lA | Γ ||- A ].
 Proof.
@@ -308,15 +255,15 @@ Proof.
     3,4,5: tea.
     + exact IHdom.
     + intros Δ a ρ tΔ ra. eapply IHcod.
-      destruct (LRIrrelevantPreds@{i j k l i' j' k' l'} IH Δ (dom⟨ρ⟩) (dom⟨ρ⟩)
+      destruct (LRIrrelevantPreds IH Δ (dom⟨ρ⟩) (dom⟨ρ⟩)
                   (domAd Δ ρ tΔ) (IHdom Δ ρ tΔ : LRPackAdequate (LogRel@{i' j' k' l'} lA) (IHdom Δ ρ tΔ))
                   (LRTyEqRefl (domAd Δ ρ tΔ))) as [_ irrTmRed _].
       eapply (snd (irrTmRed a)). exact ra.
     + cbn. intros Δ a b ρ tΔ ra rb rab.
-      destruct (LRIrrelevantPreds@{i j k l i' j' k' l'} IH Δ (dom⟨ρ⟩) (dom⟨ρ⟩)
+      destruct (LRIrrelevantPreds IH Δ (dom⟨ρ⟩) (dom⟨ρ⟩)
                   (domAd Δ ρ tΔ) (IHdom Δ ρ tΔ : LRPackAdequate (LogRel@{i' j' k' l'} lA) (IHdom Δ ρ tΔ))
                   (LRTyEqRefl (domAd Δ ρ tΔ))) as [_ irrTmRed irrTmEq].
-      destruct (LRIrrelevantPreds@{i j k l i' j' k' l'} IH Δ (cod[a .: ρ >> tRel]) (cod[a .: ρ >> tRel])
+      destruct (LRIrrelevantPreds IH Δ (cod[a .: ρ >> tRel]) (cod[a .: ρ >> tRel])
                   (codAd Δ a ρ tΔ (snd (irrTmRed a) ra))
                   (IHcod Δ a ρ tΔ (snd (irrTmRed a) ra)
                     : LRPackAdequate (LogRel@{i' j' k' l'} lA) (IHcod Δ a ρ tΔ (snd (irrTmRed a) ra)))
@@ -328,30 +275,25 @@ Proof.
       exact (snd (irrTmEq a b) rab).
 Qed.
 
-Lemma IrrRec0@{i j k i' j' k'} l0 (ltA : l0 << zero) (ltA' : l0 << zero)
-  : prod@{v v}
-      (forall Γ t, [ LogRelRec@{i j k} zero l0 ltA | Γ ||- t ] <≈> [ LogRelRec@{i' j' k'} zero l0 ltA' | Γ ||- t ])
-      (forall Γ t (lr1 : [ LogRelRec@{i j k} zero l0 ltA | Γ ||- t ])
-              (lr2 : [ LogRelRec@{i' j' k'} zero l0 ltA' | Γ ||- t ]) u
-        , [ LogRelRec@{i j k} zero l0 ltA | Γ ||- t ≅ u | lr1 ] <≈> [ LogRelRec@{i' j' k'} zero l0 ltA' | Γ ||- t ≅ u | lr2 ]).
+
+Lemma IrrRec0 : IHStatement zero zero.
 Proof.
-  inversion ltA.
+  intros ? ltA; inversion ltA.
 Qed.
 
-Theorem IrrRec@{i j k i' j' k'} {lA} {lA'} l0 (ltA : l0 << lA) (ltA' : l0 << lA')
-  : prod@{v v}
-      (forall Γ t, [ LogRelRec@{i j k} lA l0 ltA | Γ ||- t ] <≈> [ LogRelRec@{i' j' k'} lA' l0 ltA' | Γ ||- t ])
-      (forall Γ t (lr1 : [ LogRelRec@{i j k} lA l0 ltA | Γ ||- t ])
-              (lr2 : [ LogRelRec@{i' j' k'} lA' l0 ltA' | Γ ||- t ]) u
-        , [ LogRelRec@{i j k} lA l0 ltA | Γ ||- t ≅ u | lr1 ] <≈> [ LogRelRec@{i' j' k'} lA' l0 ltA' | Γ ||- t ≅ u | lr2 ]).
+End LRIrrelevantInductionStep.
+
+Theorem IrrRec@{i j k l i' j' k' l'} {lA} {lA'} :
+  IHStatement@{i j k l i' j' k' l'} lA lA'.
 Proof.
+  intros l0 ltA ltA'.
   destruct ltA. destruct ltA'. cbn in *.
   split.
   - intros Γ t. split.
-    + eapply (LRIrrelevantCumTy@{u i j k u i' j' k'} IrrRec0@{u i j u i' j'}).
-    + eapply (LRIrrelevantCumTy@{u i' j' k' u i j k} IrrRec0@{u i' j' u i j}).
+    + eapply (LRIrrelevantCumTy@{u i j k u i' j' k'} IrrRec0@{u i j k u i' j' k'}).
+    + eapply (LRIrrelevantCumTy@{u i' j' k' u i j k} IrrRec0@{u i' j' k' u i j k}).
   - intros Γ t lr1 lr2 u.
-    destruct (LRIrrelevantPreds@{u i j k u i' j' k'} IrrRec0@{u i j u i' j'} Γ t t
+    destruct (LRIrrelevantPreds@{u i j k u i' j' k'} IrrRec0@{u i j k u i' j' k'} Γ t t
                 (lr1 : LRPackAdequate (LogRel@{u i j k} zero) lr1)
                 (lr2 : LRPackAdequate (LogRel@{u i' j' k'} zero) lr2)
                 (LRTyEqRefl_ lr1)) as [tyEq _ _].
@@ -550,10 +492,15 @@ Qed.
 
 Set Printing Primitive Projection Parameters.
 
+Lemma NeNfEqSym {Γ k k' A} : [Γ ||-NeNf k ≅ k' : A] -> [Γ ||-NeNf k' ≅ k : A].
+Proof.
+  intros []; constructor; tea; now symmetry.
+Qed.
+
 Lemma LRTmEqSym@{h i j k l} lA Γ A (lrA : [LogRel@{i j k l} lA | Γ ||- A]) : forall t u,
   [Γ ||-<lA> t ≅ u : A |lrA] -> [Γ ||-<lA> u ≅ t : A |lrA].
 Proof.
-  pattern lA, Γ, A, lrA. apply LR_rect_TyUr.
+  pattern lA, Γ, A, lrA. apply LR_rect_TyUr; clear lA Γ A lrA.
   - intros * []. unshelve econstructor; try eassumption.
     1: symmetry; eassumption.
     (* Need an additional universe level h < i *)
