theories/LogicalRelation/Induction.v
@@ -8,16 +8,10 @@ Section Inductions.
     `{!WfContext ta} `{!WfType ta} `{!Typing ta}
     `{!ConvType ta} `{!ConvTerm ta} `{!ConvNeuConv ta}
     `{!RedType ta} `{!RedTerm ta}.
-
+  
   Fixpoint LR_embedding@{i j k l} {l l'} (l_ : l << l')
     {Γ A rEq rTe rTeEq} (lr : LogRel@{i j k l} l Γ A rEq rTe rTeEq) {struct lr} : (LogRel@{i j k l} l' Γ A rEq rTe rTeEq) :=
-    match lr with
-    | LRU _ H =>
-        match
-          (match l_ with Oi => fun H' => elim H'.(URedTy.lt) end H)
-        with end
-    | LRne _ neA => LRne _ neA
-    | LRPi _ ΠA ΠAad => LRPi _ ΠA
+    let embedΠad {Γ A} {ΠA : [Γ ||-Πd A]} (ΠAad : PiRedTyAdequate _ ΠA) :=
         {|
           PiRedTy.domAd :=
             fun (Δ : context) (ρ : Δ ≤ _) (h : [  |- Δ]) => LR_embedding l_ (ΠAad.(PiRedTy.domAd) ρ h) ;
@@ -26,7 +20,22 @@ Section Inductions.
               (ha : [PiRedTy.domRed ΠA ρ h | Δ ||- a : _]) =>
             LR_embedding l_ (ΠAad.(PiRedTy.codAd) ρ h ha)
         |}
+    in
+    match lr with
+    | LRU _ H =>
+        match
+          (match l_ with Oi => fun H' => elim H'.(URedTy.lt) end H)
+        with end
+    | LRne _ neA => LRne _ neA
+    | LRPi _ ΠA ΠAad => LRPi _ ΠA (embedΠad ΠAad)
     end.
+
+  Notation PiHyp P Γ ΠA HAad G :=
+    ((forall {Δ} (ρ : Δ ≤ Γ) (h : [ |- Δ]),
+        P (HAad.(PiRedTy.domAd) ρ h)) ->
+      (forall {Δ a} (ρ : Δ ≤ Γ) (h : [ |- Δ ]) 
+        (ha : [ ΠA.(PiRedTy.domRed) ρ h | Δ ||- a : ΠA.(PiRedTy.dom)⟨ρ⟩ ]),
+        P (HAad.(PiRedTy.codAd) ρ h ha)) -> G).
 
   Theorem LR_rect@{i j k o}
     (l : TypeLevel)
@@ -41,12 +50,7 @@ Section Inductions.
       P (LRne rec neA)) -> 
 
     (forall (Γ : context) (A : term) (ΠA : PiRedTy@{j} Γ A) (HAad : PiRedTyAdequate (LR rec) ΠA),
-    (forall {Δ} (ρ : Δ ≤ Γ) (h : [ |- Δ]),
-      P (HAad.(PiRedTy.domAd) ρ h)) ->
-    (forall {Δ a} (ρ : Δ ≤ Γ) (h : [ |- Δ ]) 
-      (ha : [ ΠA.(PiRedTy.domRed) ρ h | Δ ||- a : ΠA.(PiRedTy.dom)⟨ρ⟩ ]),
-    P (HAad.(PiRedTy.codAd) ρ h ha)) ->
-    P (LRPi rec ΠA HAad)) ->
+      PiHyp P Γ ΠA HAad (P (LRPi rec ΠA HAad))) ->
 
     forall (Γ : context) (t : term) (rEq rTe : term -> Type@{j})
       (rTeEq  : term -> term -> Type@{j}) (lr : LR@{i j k} rec Γ t rEq rTe rTeEq),
@@ -62,57 +66,14 @@ Section Inductions.
       all: intros ; eapply HRec.
   Defined.
 
-  Lemma LR_rect_Π_eq@{i j k o}
-    (l : TypeLevel)
-    (rec : forall l', l' << l -> RedRel@{i j})
-    (P : forall {c t rEq rTe rTeEq},
-      LR@{i j k} rec c t rEq rTe rTeEq  -> Type@{o})
-    (hU : forall (Γ : context) A (h : [Γ ||-U<l> A]), P (LRU rec h))
-    (hne : forall (Γ : context) (A : term) (neA : [Γ ||-ne A]), P (LRne rec neA))
-    (hΠ : forall (Γ : context) (A : term) (ΠA : PiRedTy@{j} Γ A) (HAad : PiRedTyAdequate (LR rec) ΠA),
-      (forall {Δ} (ρ : Δ ≤ Γ) (h : [ |- Δ]), P (HAad.(PiRedTy.domAd) ρ h)) ->
-      (forall {Δ a} (ρ : Δ ≤ Γ) (h : [ |- Δ ]) (ha : [ ΠA.(PiRedTy.domRed) ρ h | Δ ||- a : ΠA.(PiRedTy.dom)⟨ρ⟩ ]),
-      P (HAad.(PiRedTy.codAd) ρ h ha)) ->
-      P (LRPi rec ΠA HAad)) :
-    forall (Γ : context) (A : term) (ΠA : PiRedTy@{j} Γ A) (HAad : PiRedTyAdequate (LR rec) ΠA),
-    let ihdom {Δ} (ρ : Δ ≤ Γ) (h : [ |- Δ]) : P (HAad.(PiRedTy.domAd) ρ h) :=
-      LR_rect l rec (@P) hU hne hΠ _ _ _ _ _ (HAad.(PiRedTy.domAd) ρ h)
-    in
-    let ihcod {Δ a} (ρ : Δ ≤ Γ) (h : [ |- Δ ]) (ha : [ ΠA.(PiRedTy.domRed) ρ h | Δ ||- a : ΠA.(PiRedTy.dom)⟨ρ⟩ ])
-      : P (HAad.(PiRedTy.codAd) ρ h ha) :=
-      LR_rect l rec (@P) hU hne hΠ _ _ _ _ _ (HAad.(PiRedTy.codAd) ρ h ha)
-    in
-    LR_rect l rec (@P) hU hne hΠ Γ A _ _ _ (LRPi rec ΠA HAad) = hΠ Γ A ΠA HAad (@ihdom) (@ihcod).
-  Proof. intros; reflexivity. Qed.
-
-
-  Theorem LR_rec@{i j k}
-    (l : TypeLevel)
-    (rec : forall l', l' << l -> RedRel@{i j})
-    (P : forall {c t rEq rTe rTeEq},
-      LR@{i j k} rec c t rEq rTe rTeEq  -> Set) :
-
-    (forall (Γ : context) A (h : [Γ ||-U<l> A]),
-      P (LRU rec h)) ->
-
-    (forall (Γ : context) (A : term) (neA : [Γ ||-ne A]),
-      P (LRne rec neA)) ->
-
-    (forall (Γ : context) (A : term) (ΠA : PiRedTy@{j} Γ A) (HAad : PiRedTyAdequate (LR rec) ΠA),
-    (forall {Δ} (ρ : Δ ≤ Γ) (h : [ |- Δ]),
-      P (HAad.(PiRedTy.domAd) ρ h)) ->
+  Definition LR_rec@{i j k} := LR_rect@{i j k Set}.
+  
+  Notation PiHypLogRel P Γ ΠA G :=
+    ((forall {Δ} (ρ : Δ ≤ Γ) (h : [ |- Δ]), P (ΠA.(PiRedTyPack.domRed) ρ h).(LRAd.adequate)) ->
     (forall {Δ a} (ρ : Δ ≤ Γ) (h : [ |- Δ ]) 
-      (ha : [ ΠA.(PiRedTy.domRed) ρ h | Δ ||- a : ΠA.(PiRedTy.dom)⟨ρ⟩ ]),
-    P (HAad.(PiRedTy.codAd) ρ h ha)) ->
-    P (LRPi rec ΠA HAad)) ->
+      (ha : [ Δ ||-< _ > a : ΠA.(PiRedTyPack.dom)⟨ρ⟩ |  ΠA.(PiRedTyPack.domRed) ρ h ]),
+      P (ΠA.(PiRedTyPack.codRed) ρ h ha).(LRAd.adequate)) -> G).
 
-    forall (Γ : context) (t : term) (rEq rTe : term -> Type@{j})
-      (rTeEq  : term -> term -> Type@{j}) (lr : LR@{i j k} rec Γ t rEq rTe rTeEq),
-      P lr.
-  Proof.
-    intros.
-    now apply LR_rect.
-  Defined.
 
   Theorem LR_rect_LogRelRec@{i j k l o}
     (P : forall {l Γ t rEq rTe rTeEq},
@@ -124,51 +85,18 @@ Section Inductions.
     (forall (l : TypeLevel) (Γ : context) (A : term) (neA : [Γ ||-ne A]),
       P (LRne (LogRelRec l) neA)) ->
 
-    (forall (l : TypeLevel) (Γ : context) (A : term) (ΠA : PiRedTy@{k} Γ A)
-      (HAad : PiRedTyAdequate (LogRel l) ΠA),
-    (forall {Δ} (ρ : Δ ≤ Γ) (h : [ |- Δ]),
-      P (HAad.(PiRedTy.domAd) ρ h)) ->
-    (forall {Δ a} (ρ : Δ ≤ Γ) (h : [ |- Δ ]) 
-      (ha : [ ΠA.(PiRedTy.domRed) ρ h | Δ ||- a : ΠA.(PiRedTy.dom)⟨ρ⟩ ]),
-    P (HAad.(PiRedTy.codAd) ρ h ha)) ->
-    P (LRPi (LogRelRec l) ΠA HAad)) ->
+    (forall (l : TypeLevel) (Γ : context) (A : term) (ΠA : PiRedTyPack@{i j k l} Γ A l),
+      PiHypLogRel P Γ ΠA (P (LRPi' ΠA).(LRAd.adequate ))) ->
 
     forall (l : TypeLevel) (Γ : context) (t : term) (rEq rTe : term -> Type@{k})
       (rTeEq  : term -> term -> Type@{k}) (lr : LR@{j k l} (LogRelRec@{i j k} l) Γ t rEq rTe rTeEq),
       P lr.
   Proof.
-    intros.
-    eapply LR_rect@{j k l o}; auto.
-    (* - intros. clear lr. (* this is important for unfold equations *) destruct l.
-      2: auto.
-      destruct (elim (URedTy.lt h)).
-    - auto.
-    - auto. *)
+    intros HU Hne HPi **; eapply LR_rect@{j k l o}.
+    1,2: auto.
+    - intros; eapply (HPi _ _ _ (PiRedTyPack.pack ΠA HAad)); eauto.
   Defined.
 
-  Lemma LR_rect_LogRelRecΠ_eq@{i j k l o}
-    (P : forall {l Γ t rEq rTe rTeEq}, LogRel@{i j k l} l Γ t rEq rTe rTeEq -> Type@{o})
-    (hU : forall l (Γ : context) A (h : [Γ ||-U<l> A]), P (LRU (LogRelRec l) h))
-    (hne : forall (l : TypeLevel) (Γ : context) (A : term) (neA : [Γ ||-ne A]), P (LRne (LogRelRec l) neA))
-
-    (hΠ : forall (l : TypeLevel) (Γ : context) (A : term) (ΠA : PiRedTy@{k} Γ A) 
-      (HAad : PiRedTyAdequate (LogRel l) ΠA)
-      (ihdom : forall {Δ} (ρ : Δ ≤ Γ) (h : [ |- Δ]), P (HAad.(PiRedTy.domAd) ρ h))
-      (ihcod : forall {Δ a} (ρ : Δ ≤ Γ) (h : [ |- Δ ]) (ha : [ ΠA.(PiRedTy.domRed) ρ h | Δ ||- a : ΠA.(PiRedTy.dom)⟨ρ⟩ ]),
-        P (HAad.(PiRedTy.codAd) ρ h ha)),
-    P (LRPi (LogRelRec l) ΠA HAad)) :
-    forall (l : TypeLevel) (Γ : context) (A : term) (ΠA : PiRedTy@{k} Γ A) 
-      (HAad : PiRedTyAdequate (LogRel l) ΠA),
-      let ihdom {Δ} (ρ : Δ ≤ Γ) (h : [ |- Δ]) : P (HAad.(PiRedTy.domAd) ρ h) :=
-        LR_rect_LogRelRec (@P) hU hne hΠ _ _ _ _ _ _ (HAad.(PiRedTy.domAd) ρ h)
-      in
-      let ihcod {Δ a} (ρ : Δ ≤ Γ) (h : [ |- Δ ]) (ha : [ ΠA.(PiRedTy.domRed) ρ h | Δ ||- a : ΠA.(PiRedTy.dom)⟨ρ⟩ ]) :
-        P (HAad.(PiRedTy.codAd) ρ h ha) :=
-        LR_rect_LogRelRec (@P) hU hne hΠ _ _ _ _ _ _ (HAad.(PiRedTy.codAd) ρ h ha)
-      in
-      LR_rect_LogRelRec (@P) hU hne hΠ _ _ _ _ _ _ (LRPi (LogRelRec l) ΠA HAad) =
-      hΠ l Γ A ΠA HAad (@ihdom) (@ihcod).
-  Proof. reflexivity. Qed. 
 
   Theorem LR_rect_TyUr@{i j k l o}
     (P : forall {l Γ A}, [LogRel@{i j k l} l | Γ ||- A] -> Type@{o}) :
@@ -184,47 +112,22 @@ Section Inductions.
       (forall {Δ a} (ρ : Δ ≤ Γ) (h : [ |- Δ ]) 
        (ha : [ ΠA.(PiRedTyPack.domRed) ρ h | Δ ||- a : ΠA.(PiRedTyPack.dom)⟨ρ⟩ ]),
       P (ΠA.(PiRedTyPack.codRed) ρ h ha)) ->
-    P (LRPi' l ΠA)) ->
-    (* (forall (l : TypeLevel) (Γ : context) (A : term) (ΠA : PiRedTy@{k} Γ A) (HAad : PiRedTyAdequate (LogRel l) ΠA),
-    (forall {Δ} (ρ : Δ ≤ Γ) (h : [ |- Δ]),
-      P (LRbuild (HAad.(PiRedTy.domAd) ρ h))) ->
-    (forall {Δ a} (ρ : Δ ≤ Γ) (h : [ |- Δ ]) 
-      (ha : [ ΠA.(PiRedTy.domRed) ρ h | Δ ||- a : ΠA.(PiRedTy.dom)⟨ρ⟩ ]),
-    P (LRbuild (HAad.(PiRedTy.codAd) ρ h ha))) ->
-    P (LRPi_ l ΠA HAad)) -> *)
+    P (LRPi' ΠA)) ->
 
     forall (l : TypeLevel) (Γ : context) (A : term) (lr : [LogRel@{i j k l} l | Γ ||- A]),
       P lr.
   Proof.
     intros HU Hne HPi l Γ A lr.
     apply (LR_rect_LogRelRec@{i j k l o} (fun l Γ A _ _ _ lr => P l Γ A (LRbuild lr))).
-    1,2: auto.
-    intros; eapply (HPi _ _ _ (PiRedTyPack.pack ΠA HAad)); eauto.    
+    1-3: auto.
   Defined.
 
-  Theorem LR_rect_TyUr_Π_eq@{i j k l o}
-    (P : forall {l Γ A}, [LogRel@{i j k l} l | Γ ||- A] -> Type@{o})
-    (hU : forall l (Γ : context) A (h : [Γ ||-U<l> A]), P (LRU_ h))
-    (hne : forall (l : TypeLevel) (Γ : context) (A : term) (neA : [Γ ||-ne A]), P (LRne_ l neA))
-    (hΠ : forall (l : TypeLevel) (Γ : context) (A : term) (ΠA : PiRedTyPack@{i j k l} Γ A l)
-      (ihdom : forall {Δ} (ρ : Δ ≤ Γ) (h : [ |- Δ]), P (ΠA.(PiRedTyPack.domRed) ρ h))
-      (ihcod : forall {Δ a} (ρ : Δ ≤ Γ) (h : [ |- Δ ]) 
-        (ha : [ ΠA.(PiRedTyPack.domRed) ρ h | Δ ||- a : ΠA.(PiRedTyPack.dom)⟨ρ⟩ ]),
-        P (ΠA.(PiRedTyPack.codRed) ρ h ha)),
-      P (LRPi' l ΠA)) :
-    forall (l : TypeLevel) (Γ : context) (A : term) (ΠA : PiRedTyPack@{i j k l} Γ A l),
-      let ihdom {Δ} (ρ : Δ ≤ Γ) (h : [ |- Δ]) : P (ΠA.(PiRedTyPack.domRed) ρ h) :=
-        LR_rect_TyUr (@P) hU hne hΠ _ _ _ (ΠA.(PiRedTyPack.domRed) ρ h)
-      in
-      let ihcod {Δ a} (ρ : Δ ≤ Γ) (h : [ |- Δ ]) 
-        (ha : [ ΠA.(PiRedTyPack.domRed) ρ h | Δ ||- a : ΠA.(PiRedTyPack.dom)⟨ρ⟩ ]) :
-        P (ΠA.(PiRedTyPack.codRed) ρ h ha) :=
-        LR_rect_TyUr (@P) hU hne hΠ _ _ _ (ΠA.(PiRedTyPack.codRed) ρ h ha)
-      in
-      LR_rect_TyUr (@P) hU hne hΠ _ _ _ (LRPi' l ΠA) = hΠ l Γ A ΠA (@ihdom) (@ihcod).
-    Proof.
-      reflexivity.
-    Qed. 
+  Notation PiHyp0 P Γ ΠA HAad G :=
+    ((forall {Δ} (ρ : Δ ≤ Γ) (h : [ |- Δ]),
+        P (HAad.(PiRedTy.domAd) ρ h)) ->
+      (forall {Δ a} (ρ : Δ ≤ Γ) (h : [ |- Δ ]) 
+        (ha : [ ΠA.(PiRedTy.domRed) ρ h | Δ ||- a : ΠA.(PiRedTy.dom)⟨ρ⟩ ]),
+        P (HAad.(PiRedTy.codAd) ρ h ha)) -> G).
 
 
   (* Induction principle specialized at level 0 to minimize universe constraints *)
@@ -235,14 +138,9 @@ Section Inductions.
 
     (forall (Γ : context) (A : term) (neA : [Γ ||-ne A]),
       P (LRne rec0 neA)) -> 
-
-    (forall (Γ : context) (A : term) (ΠA : PiRedTy@{j} Γ A) (HAad : PiRedTyAdequate (LogRel0@{i j k}) ΠA),
-    (forall {Δ} (ρ : Δ ≤ Γ) (h : [ |- Δ]),
-      P (HAad.(PiRedTy.domAd) ρ h)) ->
-    (forall {Δ a} (ρ : Δ ≤ Γ) (h : [ |- Δ ]) 
-      (ha : [ ΠA.(PiRedTy.domRed) ρ h | Δ ||- a : ΠA.(PiRedTy.dom)⟨ρ⟩ ]),
-    P (HAad.(PiRedTy.codAd) ρ h ha)) ->
-    P (LRPi rec0 ΠA HAad)) ->
+    
+    (forall (Γ : context) (A : term) (ΠA : PiRedTy@{j} Γ A) (HAad : PiRedTyAdequate LogRel0@{i j k} ΠA),
+      PiHyp0 P Γ ΠA HAad (P (LRPi rec0 ΠA HAad))) ->
 
     forall (Γ : context) (t : term) (rEq rTe : term -> Type@{j})
       (rTeEq  : term -> term -> Type@{j}) (lr : LogRel0@{i j k} Γ t rEq rTe rTeEq),
@@ -254,33 +152,11 @@ Section Inductions.
     destruct lr.
     - destruct H as [? lt]; destruct (elim lt).
     - eapply Hne.
-    - eapply HPi.
-      all: intros ; eapply HRec.
-  Defined.
-
-  Theorem LR_rect_TyUr0@{i j k o}
-    (P : forall {Γ A}, [LogRel0@{i j k} | Γ ||- A] -> Type@{o}) :
-
-    (forall (Γ : context) (A : term) (neA : [Γ ||-ne A]),
-      P (LRbuild0@{i j k} (LRne@{i j k} rec0 neA))) ->
-
-    (forall (Γ : context) (A : term) (ΠA : PiRedTy@{j} Γ A) (HAad : PiRedTyAdequate LogRel0 ΠA),
-    (forall {Δ} (ρ : Δ ≤ Γ) (h : [ |- Δ]),
-      P (LRbuild0@{i j k} (HAad.(PiRedTy.domAd) ρ h))) ->
-    (forall {Δ a} (ρ : Δ ≤ Γ) (h : [ |- Δ ]) 
-      (ha : [ ΠA.(PiRedTy.domRed) ρ h | Δ ||- a : ΠA.(PiRedTy.dom)⟨ρ⟩ ]),
-    P (LRbuild0@{i j k} (HAad.(PiRedTy.codAd) ρ h ha))) ->
-    P (LRbuild0@{i j k} (LRPi rec0 ΠA HAad))) ->
-
-    forall (Γ : context) (A : term) (lr : [LogRel0@{i j k} | Γ ||- A]),
-      P lr.
-  Proof.
-    intros Hne HPi Γ A lr.
-    apply (LR_rect0 (fun Γ A _ _ _ lr => P Γ A (LRbuild0 lr))).
-    all: auto.
+    - eapply HPi; intros ; eapply HRec.
   Defined.
 
 End Inductions.
+
 
 Section Inversions.
   Context `{ta : tag}
@@ -299,11 +175,11 @@ Section Inversions.
     pattern l, Γ, A, lr; eapply LR_rect_TyUr; clear l Γ A lr.
     + intros * h whA.
       epose proof (redtywf_whnf (URedTy.red h) whA); subst; assumption.
-    + intros * h whA. pose (h' := h); destruct h' as [ty [?? r] ne].
-      pose proof (redty_whnf r whA); subst.
+    + intros * h whA. pose (h' := h); destruct h' as [ty r ne].
+      pose proof (redtywf_whnf r whA); subst.
       destruct ty; inversion ne; eassumption.
-    + intros ??? h _ _ whA. pose (h' := h); destruct h' as [??? [?? r]].
-      pose proof (redty_whnf r whA); subst. eassumption.
+    + intros ??? h _ _ whA. pose (h' := h); destruct h' as [??? r].
+      pose proof (redtywf_whnf r whA); subst. eassumption.
   Qed.
 
   Lemma invLRU {Γ l} : [Γ ||-<l> U] -> [Γ ||-U<l> U].
